clean up eqdec instances

deps/poulet4/lib/P4automata/Examples.v
@@ -1,12 +1,31 @@
+Require Coq.Classes.EquivDec.
+Require Import Coq.Program.Program.
 Require Import Poulet4.P4automata.Syntax.
 Require Import Poulet4.P4automata.Sum.
 Require Import Poulet4.P4automata.PreBisimulationSyntax.
+
+Ltac prep_equiv :=
+  unfold Equivalence.equiv, RelationClasses.complement in *;
+  program_simpl; try congruence.
+
+Obligation Tactic := prep_equiv.
+
 Module Simple.
-  Inductive state :=
+  Inductive state: Type :=
   | Start.
 
-  Inductive header :=
+  Program Instance state_eq_dec: EquivDec.EqDec state eq :=
+    fun x y => match x, y with
+            | Start, Start => in_left
+            end.
+
+  Inductive header: Type :=
   | HdrSimple.
+
+  Global Program Instance header_eq_dec: EquivDec.EqDec header eq :=
+    fun x y => match x, y with
+            | HdrSimple, HdrSimple => in_left
+            end.
 
   Definition st_start: Syntax.state state header :=
     {| st_op := OpExtract 16 (HRVar HdrSimple);
@@ -17,13 +36,29 @@ Module Simple.
 End Simple. 
 
 Module Split.
-  Inductive state :=
+  Inductive state: Type :=
   | StSplit1
   | StSplit2.
 
-  Inductive header :=
+  Program Instance state_eq_dec: EquivDec.EqDec state eq :=
+    fun x y => match x, y with
+            | StSplit1, StSplit1
+            | StSplit2, StSplit2 => in_left
+            | _, _ => in_right
+            end.
+  Solve Obligations with prep_equiv; try destruct x; destruct y; intuition congruence.
+
+  Inductive header: Type :=
   | HdrSplit1
   | HdrSplit2.
+
+  Global Program Instance header_eq_dec: EquivDec.EqDec header eq :=
+    fun x y => match x, y with
+            | HdrSplit1, HdrSplit1
+            | HdrSplit2, HdrSplit2 => in_left
+            | _, _ => in_right
+            end.
+  Solve Obligations with prep_equiv; try destruct x; destruct y; intuition congruence.
 
   Definition st_split1: Syntax.state state header :=
     {| st_op := OpExtract 8 (HRVar HdrSplit1);
@@ -38,7 +73,14 @@ Module Split.
 End Split.
 
 Module SimpleSplit.
+  Definition state: Type := Sum.S Simple.state Split.state.
+  Instance state_eq_dec: EquivDec.EqDec state eq :=
+    ltac:(typeclasses eauto).
+
+  Definition header := Sum.H Simple.header Split.header.
+  Instance header_eq_dec: EquivDec.EqDec state eq :=
+    ltac:(typeclasses eauto).
+
   Definition aut := Eval cbv in sum Simple.aut Split.aut.
-  Print aut.
 End SimpleSplit.
 
